WIP

src/gopt/AssertInsertion.v
@@ -31,6 +31,17 @@ Require Import GSimulation.
 Set Implicit Arguments.
 
 
+Inductive opt_lang_step: forall (e:ProgramEvent.t) (st1 st2:State.t), Prop :=
+| opt_lang_step_none
+    st:
+    opt_lang_step ProgramEvent.silent st st
+| opt_lang_step_some
+    e st1 st2
+    (STEP: lang.(Language.step) e st1 st2):
+    opt_lang_step e st1 st2
+.
+
+
 Section AssertInsertion.
   Variable
     (S:ThreadsProp)
@@ -53,9 +64,10 @@ Section AssertInsertion.
       cond
       stmts1_src stmts2_src stmts_src
       stmts1_tgt stmts2_tgt stmts_tgt
-      (SIM1: sim_stmts tid stmts1_src stmts1_tgt)
-      (SIM2: sim_stmts tid stmts2_src stmts2_tgt)
-      (SIM: sim_stmts tid stmts_src stmts_tgt):
+      (* (SIM1: sim_stmts tid stmts1_src stmts1_tgt) *)
+      (* (SIM2: sim_stmts tid stmts2_src stmts2_tgt) *)
+      (SIM1: sim_stmts tid (stmts1_src ++ stmts_src) (stmts1_tgt ++ stmts_tgt))
+      (SIM2: sim_stmts tid (stmts2_src ++ stmts_src) (stmts2_tgt ++ stmts_tgt)):
       sim_stmts tid
                 ((Stmt.ite cond stmts1_src stmts2_src)::stmts_src)
                 ((Stmt.ite cond stmts1_tgt stmts2_tgt)::stmts_tgt)
@@ -63,8 +75,9 @@ Section AssertInsertion.
       cond
       stmts1_src stmts_src
       stmts1_tgt stmts_tgt
-      (SIM1: sim_stmts tid stmts1_src stmts1_tgt)
-      (SIM: sim_stmts tid stmts_src stmts_tgt):
+      (SIM: sim_stmts tid
+                      (stmts1_src ++ (Stmt.ite cond ((Stmt.dowhile stmts1_src cond)::nil) nil) :: stmts_src)
+                      (stmts1_tgt ++ (Stmt.ite cond ((Stmt.dowhile stmts1_tgt cond)::nil) nil) :: stmts_tgt)):
       sim_stmts tid
                 ((Stmt.dowhile stmts1_src cond)::stmts_src)
                 ((Stmt.dowhile stmts1_tgt cond)::stmts_tgt)
@@ -80,7 +93,7 @@ Section AssertInsertion.
   Inductive sim_state (tid: Ident.t) (st_src st_tgt: State.t): Prop :=
   | sim_state_intro
       (STMTS: sim_stmts tid st_src.(State.stmts) st_tgt.(State.stmts))
-      (REGS: forall reg, st_src.(State.regs) reg = st_tgt.(State.regs) reg)
+      (REGS: st_src.(State.regs) = st_tgt.(State.regs))
   .
   Hint Constructors sim_state.
 
@@ -92,6 +105,122 @@ Section AssertInsertion.
       (MEMORY: e_src.(Thread.memory) = e_tgt.(Thread.memory))
   .
   Hint Constructors sim_thread.
+
+
+  Lemma sim_state_step
+        tid st1_src
+        e st1_tgt st2_tgt
+        (SIM1: sim_state tid st1_src st1_tgt)
+        (STEP: lang.(Language.step) e st1_tgt st2_tgt)
+        (EVENT: e <> ProgramEvent.abort):
+    exists st2_src,
+      <<STEP_SRC: opt_lang_step e st1_src st2_src>> /\
+      <<SIM2: sim_state tid st2_src st2_tgt>>.
+  Proof.
+    destruct st1_src, st1_tgt, st2_tgt.
+    inv SIM1. ss. subst.
+    inv STMTS.
+    - inv STEP.
+    - exists (State.mk regs1 stmts_src).
+      inv STEP. split; eauto.
+      econs 2. econs; eauto.
+    - inv STEP. esplits.
+      + econs 2. econs; eauto.
+      + condtac; eauto.
+    - inv STEP. esplits.
+      + econs 2. econs; eauto.
+      + ss.
+    - inv STEP; inv INSTR; ss. esplits.
+      + econs 1.
+      + ss.
+  Qed.
+
+  Lemma sim_thread_abort_step
+        tid e1_src
+        pf e1_tgt e2_tgt
+        (SEM: S tid lang e1_src.(Thread.state))
+        (SIM1: sim_thread tid e1_src e1_tgt)
+        (STEP_TGT: Thread.step pf ThreadEvent.abort e1_tgt e2_tgt):
+    False \/
+    exists e2_src,
+      <<STEP_SRC: Thread.step pf ThreadEvent.abort e1_src e2_src>> /\
+      <<SIM2: sim_thread tid e2_src e2_tgt>>.
+  Proof.
+    destruct e1_src, e1_tgt, e2_tgt. ss.
+    inv SIM1. ss. subst.
+    destruct state, state0. inv STATE. ss. subst.
+    inv STEP_TGT; inv STEP; ss.
+    inv STATE. inv INSTR. inv STMTS.
+    - right. esplits.
+      + econs 2. econs; eauto. ss. econs; eauto. econs; eauto.
+      + econs; eauto.
+    - left. eapply SUCCESS; eauto.
+  Qed.
+
+  Lemma sim_thread_step
+        tid e1_src
+        pf e e1_tgt e2_tgt
+        (SIM1: sim_thread tid e1_src e1_tgt)
+        (STEP_TGT: Thread.step pf e e1_tgt e2_tgt)
+        (EVENT: e <> ThreadEvent.abort):
+    exists e2_src,
+      <<STEP_SRC: Thread.opt_step e e1_src e2_src>> /\
+      <<SIM2: sim_thread tid e2_src e2_tgt>>.
+  Proof.
+    destruct e1_src, e1_tgt, e2_tgt. ss.
+    inv SIM1. ss. subst.
+    inv STEP_TGT; inv STEP; ss.
+    - esplits.
+      + econs 2. econs 1. econs; eauto.
+      + eauto.
+    - exploit sim_state_step; eauto.
+      { destruct e; ss. }
+      i. des.
+      inv LOCAL; inv STEP_SRC; ss.
+      + esplits.
+        * econs 1.
+        * econs; eauto.
+      + esplits.
+        * econs 2. econs 2. econs; eauto.
+        * econs; eauto.
+      + esplits.
+        * econs 2. econs 2. econs; eauto.
+        * econs; eauto.
+      + esplits.
+        * econs 2. econs 2. econs; eauto.
+        * econs; eauto.
+      + esplits.
+        * econs 2. econs 2. econs; eauto.
+        * econs; eauto.
+      + esplits.
+        * econs 2. econs 2. econs; eauto.
+        * econs; eauto.
+      + esplits.
+        * econs 2. econs 2. econs; eauto.
+        * econs; eauto.
+  Qed.
+
+  Lemma sim_thread_rtc_tau_step
+        tid e1_src e1_tgt e2_tgt
+        (SIM1: sim_thread tid e1_src e1_tgt)
+        (STEPS_TGT: rtc (@Thread.tau_step lang) e1_tgt e2_tgt):
+    exists e2_src,
+      <<STEPS_SRC: rtc (@Thread.tau_step lang) e1_src e2_src>> /\
+      <<SIM2: sim_thread tid e2_src e2_tgt>>.
+  Proof.
+    revert e1_src SIM1.
+    induction STEPS_TGT; eauto; i.
+    inv H. inv TSTEP.
+    exploit sim_thread_step; eauto.
+    { destruct e; ss. }
+    i. des.
+    exploit IHSTEPS_TGT; eauto. i. des.
+    esplits; [|eauto].
+    inv STEP_SRC; eauto.
+    econs 2; eauto.
+    econs; [econs; eauto|ss].
+  Qed.
+
 
   Inductive sim_conf (c_src c_tgt: Configuration.t): Prop :=
   | sim_conf_intro
@@ -219,10 +348,10 @@ Section AssertInsertion.
     exploit Memory.max_full_timemap_exists; try apply CLOSED_CAP. i. des.
     hexploit Memory.max_full_timemap_closed; try exact x1; eauto. intro SC_MAX.
     exploit CONSISTENT; eauto. s. i. des.
-    { (* normal certification *)
+    { (* abort certification *)
       admit.
     }
-    { (* abort certification *)
+    { (* normal certification *)
       admit.
     }
   Admitted.
